\section{Derivações}
    \begin{lemma}
        $\vdash\alpha\to\alpha$
        \begin{proof}
            Pode ser provado pela seguinte sucessão de dedução:
        
            \begin{fitch}
                \fa(\alpha\to(\alpha\to\alpha)\to\alpha)\to(\alpha\to\alpha\to\alpha)\to\alpha\to\alpha&$\mathbf{A_2}$\\
                \fa\alpha\to(\alpha\to\alpha)\to\alpha&$\mathbf{A_1}$\\
                \fa(\alpha\to\alpha\to\alpha)\to\alpha\to\alpha&$\mathbf{R_1}\;\set{1, 2}$\\
                \fa\alpha\to\alpha\to\alpha&$\mathbf{A_1}$\\
                \fa\alpha\to\alpha&$\mathbf{R_1}\;\set{3, 4}$\\
            \end{fitch}
            \vspace*{-18pt}
            \qedhere
        \end{proof}
    \end{lemma}

    \begin{lemma}
        $\vdash\bot\to\alpha$
        \begin{proof}
            Pode ser provado pela seguinte sucessão de dedução:
        
            \begin{fitch}
                \fa(((\alpha\to\bot)\to\bot)\to\alpha)\to\bot\to((\alpha\to\bot)\to\bot)\to\alpha&$\mathbf{A_1}$\\
                \fa((\alpha\to\bot)\to\bot)\to\alpha&$\mathbf{A_\neg}$\\
                \fa\bot\to((\alpha\to\bot)\to\bot)\to\alpha&$\mathbf{R_1}\;\set{1, 2}$\\
                \fa(\bot\to(\alpha\to\bot)\to\bot)\to\bot\to\bot\to(\alpha\to\bot)\to\bot&$\mathbf{A_1}$\\
                \fa\bot\to(\alpha\to\bot)\to\bot&$\mathbf{A_1}$\\
                \fa\bot\to\bot\to(\alpha\to\bot)\to\bot&$\mathbf{R_1}\;\set{4, 5}$\\
                \fa\bot\to\bot&$\mathbf{L_1}$\\
                \fa\\
                \fa\\
                \fa\bot\to(\alpha\to\bot)\to\bot\\
                \fa\\
                \fa\\
                \fa\bot\to\alpha\\
            \end{fitch}
            \vspace*{-18pt}
            \qedhere
        \end{proof}
    \end{lemma}

    \begin{lemma}
        $\vdash(\alpha\to\beta)\to(\alpha\to\gamma)\to\alpha\to\beta\wedge\gamma$.
    \end{lemma}

    \begin{lemma}
        $\vdash\nec(\alpha\wedge\beta)\to\nec\alpha\wedge\nec\beta$.

        \begin{proof}
            Pode ser provado pela seguinte sucessão de dedução:

            \begin{fitch}
                \fa\alpha\wedge\beta\to\alpha\\
                \fa\nec(\alpha\wedge\beta\to\alpha)\\
                \fa\nec(\alpha\wedge\beta\to\alpha)\to(\nec(\alpha\wedge\beta)\to\nec\alpha)\\
                \fa\nec(\alpha\wedge\beta)\to\nec\alpha\\
                \fa\alpha\wedge\beta\to\beta\\
                \fa\nec(\alpha\wedge\beta\to\beta)\\
                \fa\nec(\alpha\wedge\beta\to\beta)\to(\nec(\alpha\wedge\beta)\to\nec\beta)\\
                \fa\nec(\alpha\wedge\beta)\to\nec\beta\\
                \fa(\nec(\alpha\wedge\beta)\to\nec\alpha)\to(\nec(\alpha\wedge\beta)\to\nec\beta)\to\nec(\alpha\wedge\beta)\to\nec\alpha\wedge\nec\beta\\
                \fa(\nec(\alpha\wedge\beta)\to\nec\beta)\to\nec(\alpha\wedge\beta)\to\nec\alpha\wedge\nec\beta\\
                \fa\nec(\alpha\wedge\beta)\to\nec\alpha\wedge\nec\beta{}
            \end{fitch}
            \vspace*{-18pt}
            \qedhere
        \end{proof}
    \end{lemma}

    \begin{lemma}    
        $\vdash\nec\alpha\wedge\nec\beta\to\nec(\alpha\wedge\beta)$.
    \end{lemma}

    \begin{lemma}
        $\vdash\nec(\alpha\to\beta)\to\nec\alpha\to\beta$.
    \end{lemma}